SystemF2Effect: fix admits in type_kind
Ignore-this: ef4043c48eee3dd4bbb25d2f1f166142

darcs-hash:20130117110607-08f32-fcb3a2c2fc830b718339e70e039c961539113091

devel/Iron/Language/SystemF2Effect/Type/MaskOnVar.v
@@ -6,12 +6,12 @@ Require Import Iron.Language.SystemF2Effect.Type.KiJudge.
 
 (* Mask effects on the given region, 
    replacing with the bottom effect. *)
-Fixpoint mask (r : nat) (e : ty) : ty
+Fixpoint maskOnVar (r : nat) (e : ty) : ty
  := match e with
     |  TVar tc       => TVar tc
-    |  TForall k t1  => TForall k (mask (S r) t1)
-    |  TApp t1 t2    => TApp (mask r t1) (mask r t2)
-    |  TSum t1 t2    => TSum (mask r t1) (mask r t2)
+    |  TForall k t1  => TForall k (maskOnVar (S r) t1)
+    |  TApp t1 t2    => TApp (maskOnVar r t1) (maskOnVar r t2)
+    |  TSum t1 t2    => TSum (maskOnVar r t1) (maskOnVar r t2)
     |  TBot k        => TBot k
 
     |  TCon0 tc      => TCon0 tc
@@ -21,22 +21,22 @@ Fixpoint mask (r : nat) (e : ty) : ty
        | TVar n' 
        => if beq_nat r n' 
              then TBot KEffect 
-             else TCon1 tc (mask r t1)
+             else TCon1 tc (maskOnVar r t1)
 
-       | _ =>     TCon1 tc (mask r t1)
+       | _ =>     TCon1 tc (maskOnVar r t1)
        end
     
-    | TCon2 tc t1 t2 => TCon2 tc (mask r t1) (mask r t2)
+    | TCon2 tc t1 t2 => TCon2 tc (maskOnVar r t1) (maskOnVar r t2)
 
     | TCap  tc       => TCap tc
     end.
-Arguments mask r e : simpl nomatch.
+Arguments maskOnVar r e : simpl nomatch.
 
 
-Lemma mask_kind
+Lemma maskOnVar_kind
  :  forall ke sp t k n
  ,  KIND ke sp t k 
- -> KIND ke sp (mask n t) k.
+ -> KIND ke sp (maskOnVar n t) k.
 Proof.
  intros. gen ke sp n k.
  induction t; intros; inverts_kind; simpl; auto.
@@ -50,7 +50,7 @@ Proof.
   spec IHt H6.
   destruct t0; simpl in *; eauto.
   destruct t;  norm; inverts H4;
-  unfold mask; split_if; norm; eauto;
+  unfold maskOnVar; split_if; norm; eauto;
    eapply KiCon1; norm; eauto. 
 
  Case "TCon2".
@@ -61,9 +61,9 @@ Proof.
 Qed.
 
 
-Lemma liftTT_mask
+Lemma liftTT_maskOnVar
  :  forall r d t
- ,  mask r (liftTT 1 (1 + (r + d)) t) = liftTT 1 (1 + (r + d)) (mask r t).
+ ,  maskOnVar r (liftTT 1 (1 + (r + d)) t) = liftTT 1 (1 + (r + d)) (maskOnVar r t).
 Proof.
 Opaque le_gt_dec.
 
@@ -86,14 +86,14 @@ Opaque le_gt_dec.
   destruct t0.
 
   SCase "TVar".
-   repeat (unfold mask; simpl; split_if; norm_beq_nat; auto; try omega).
+   repeat (unfold maskOnVar; simpl; split_if; norm_beq_nat; auto; try omega).
           
   (* GAH. Most of this rubbish is just to force single step evaluation of mask.
      I can't work out how to do a 'simpl' with only a single step *)
   SCase "TForall".
    simpl liftTT.
    set     (X0 := TForall k (liftTT 1 (S (S (r + d))) t0)).
-   rrwrite (mask r (TCon1 t X0)          = TCon1 t (mask r X0)).
+   rrwrite (maskOnVar r (TCon1 t X0)        = TCon1 t (maskOnVar r X0)).
    subst X0.
    rrwrite (TForall k (liftTT 1 (S (S (r + d))) t0) = liftTT 1 (S (r + d)) (TForall k t0)).
    rewritess. simpl. auto.
@@ -101,7 +101,7 @@ Opaque le_gt_dec.
   SCase "TApp".
    simpl liftTT.
    set      (X0 := TApp (liftTT 1 (S (r + d)) t0_1) (liftTT 1 (S (r + d)) t0_2)).
-    rrwrite (mask r (TCon1 t X0)           = TCon1 t (mask r X0)).
+    rrwrite (maskOnVar r (TCon1 t X0)       = TCon1 t (maskOnVar r X0)).
    subst X0.
    rrwrite  ( TApp (liftTT 1 (S (r + d)) t0_1) (liftTT 1 (S (r + d)) t0_2)
             = liftTT 1 (S (r + d)) (TApp t0_1 t0_2)).
@@ -110,7 +110,7 @@ Opaque le_gt_dec.
   SCase "TSum".
    simpl liftTT.
    set      (X0 := TSum (liftTT 1 (S (r + d)) t0_1) (liftTT 1 (S (r + d)) t0_2)).
-    rrwrite (mask r (TCon1 t X0)           = TCon1 t (mask r X0)).
+    rrwrite (maskOnVar r (TCon1 t X0)      = TCon1 t (maskOnVar r X0)).
    subst X0.
    rrwrite  ( TSum (liftTT 1 (S (r + d)) t0_1) (liftTT 1 (S (r + d)) t0_2)
             = liftTT 1 (S (r + d)) (TSum t0_1 t0_2)).
@@ -125,7 +125,7 @@ Opaque le_gt_dec.
  SCase "TCon1".
   simpl liftTT.
   set    (X0 := TCon1 t0 (liftTT 1 (S (r + d)) t1)).
-   rrwrite (mask r (TCon1 t X0)           = TCon1 t (mask r X0)).
+   rrwrite (maskOnVar r (TCon1 t X0)       = TCon1 t (maskOnVar r X0)).
   subst X0.
   rrwrite  ( TCon1 t0 (liftTT 1 (S (r + d)) t1)
            = liftTT 1 (S (r + d)) (TCon1 t0 t1)).
@@ -134,7 +134,7 @@ Opaque le_gt_dec.
   SCase "TCon2".
    simpl liftTT.
    set      (X0 := TCon2 t0 (liftTT 1 (S (r + d)) t0_1) (liftTT 1 (S (r + d)) t0_2)).
-    rrwrite (mask r (TCon1 t X0)           = TCon1 t (mask r X0)).
+    rrwrite (maskOnVar r (TCon1 t X0)      = TCon1 t (maskOnVar r X0)).
    subst X0.
    rrwrite  ( TCon2 t0 (liftTT 1 (S (r + d)) t0_1) (liftTT 1 (S (r + d)) t0_2)
             = liftTT 1 (S (r + d)) (TCon2 t0 t0_1 t0_2)).
