devel/Iron/Language/SystemF2Effect/Value/TyJudge.v
@@ -115,8 +115,8 @@ Inductive
   (* Create a new location region. *)
   | TxNew
     :  forall ke te se sp x t tL e eL
-    ,  lowerTT 0 t          = Some tL
-    -> lowerTT 0 (mask 0 e) = Some eL
+    ,  lowerTT 0 t               = Some tL
+    -> lowerTT 0 (maskOnVar 0 e) = Some eL
     -> TYPEX (ke :> KRegion) (liftTE 0 te) (liftTE 0 se) sp x        t  e
     -> TYPEX ke              te             se           sp (XNew x) tL eL
 
